seiostar/RQ.TypingRelation.Tests.fst
@@ -45,55 +45,55 @@ open Examples
 
 let test_ut_unit
   : qUnit ⊩ ut_unit
-  = mk_dturniqet (fun _ -> Qtt)
+  = pack_turnstile Qtt
 
 let test_ut_true
   : qBool ⊩ ut_true
-  = mk_dturniqet (fun _ -> QTrue)
+  = pack_turnstile QTrue
 
 let test_ut_false
   : qBool ⊩ ut_false
-  = mk_dturniqet (fun _ -> QFalse)
+  = pack_turnstile QFalse
 
 let test_constant ()
   : ((qBool ^-> qBool) ⊩ constant)
   by (simplify_via_norm ())
-  = mk_dturniqet (fun _ -> QLambda QTrue)
+  = pack_turnstile (QLambda QTrue)
 
 let test_constant' ()
   : ((qBool ^-> qBool) ⊩ constant)
   by (simplify_via_norm ())
-  = mk_dturniqet (fun _ -> QLambda (QWeaken QTrue))
+  = pack_turnstile (QLambda (QWeaken QTrue))
 
 let test_identity ()
   : (qBool ^-> qBool) ⊩ identity
   by (simplify_via_norm ())
-  = mk_dturniqet (fun _ -> QLambda QAxiom)
+  = pack_turnstile (QLambda QAxiom)
 
 let test_thunked_id ()
   : (qBool ^-> (qBool ^-> qBool)) ⊩ thunked_id
   by (simplify_via_norm ())
-  = mk_dturniqet (fun _ -> QLambda (QLambda QAxiom))
+  = pack_turnstile (QLambda (QLambda QAxiom))
 
 let test_proj1 ()
   : (qBool ^-> qBool ^-> qBool ^-> qBool) ⊩ proj1
   by (simplify_via_norm ())
-  = mk_dturniqet (fun _ -> QLambda (QLambda (QLambda qVar2)))
+  = pack_turnstile (QLambda (QLambda (QLambda qVar2)))
 
 let test_proj2 ()
   : (qBool ^-> qBool ^-> qBool ^-> qBool) ⊩ proj2
   by (simplify_via_norm ())
-  = mk_dturniqet (fun _ -> QLambda (QLambda (QLambda qVar1)))
+  = pack_turnstile (QLambda (QLambda (QLambda qVar1)))
 
 let test_proj3 ()
   : (qBool ^-> qBool ^-> qBool ^-> qBool) ⊩ proj3
   by (simplify_via_norm ())
-  = mk_dturniqet (fun _ -> QLambda (QLambda (QLambda QAxiom)))
+  = pack_turnstile (QLambda (QLambda (QLambda QAxiom)))
 
 let test_apply_top_level_def ()
   : (qBool ^-> qBool) ⊩ apply_top_level_def
   by (simplify_via_norm ())
-  = mk_dturniqet (fun _ -> QLambda (QApp
+  = pack_turnstile (QLambda (QApp
               (QApp
                 (QLambda (QLambda QAxiom))
                 QAxiom)
@@ -102,7 +102,7 @@ let test_apply_top_level_def ()
 let test_apply_top_level_def' ()
   : (qBool ^-> qBool ^-> qBool) ⊩ apply_top_level_def'
   by (simplify_via_norm ())
-  = mk_dturniqet (fun _ -> QLambda (QLambda (QApp
+  = pack_turnstile (QLambda (QLambda (QApp
                        (QApp
                           (QLambda (QLambda QAxiom))
                           qVar1)
@@ -111,75 +111,75 @@ let test_apply_top_level_def' ()
 let test_papply__top_level_def ()
   : (qBool ^-> qBool ^-> qBool) ⊩ papply__top_level_def
   by (simplify_via_norm ())
-  = mk_dturniqet (fun _ -> QLambda (QApp
+  = pack_turnstile (QLambda (QApp
               (QLambda (QLambda QAxiom))
               QAxiom))
 
 let test_apply_arg ()
   : ((qUnit ^-> qUnit) ^-> qUnit) ⊩ apply_arg
   by (simplify_via_norm ())
-  = mk_dturniqet (fun _ -> QLambda (QApp QAxiom Qtt))
+  = pack_turnstile (QLambda (QApp QAxiom Qtt))
 
 let test_apply_arg2 ()
   : ((qBool ^-> qBool ^-> qBool) ^-> qBool) ⊩ apply_arg2
   by (simplify_via_norm ())
-  = mk_dturniqet (fun _ -> QLambda (QApp (QApp QAxiom QTrue) QFalse))
+  = pack_turnstile (QLambda (QApp (QApp QAxiom QTrue) QFalse))
 
 let test_papply_arg2 ()
   : ((qBool ^-> qBool ^-> qBool) ^-> qBool ^-> qBool) ⊩ papply_arg2
   by (simplify_via_norm ())
-  = mk_dturniqet (fun _ -> QLambda (QApp QAxiom QTrue))
+  = pack_turnstile (QLambda (QApp QAxiom QTrue))
 
 [@expect_failure]
 let test_proj2'
   : (qBool ^-> qBool ^-> qBool ^-> qBool) ⊩ proj2
-  = mk_dturniqet (fun _ -> QLambda (QLambda (QLambda QAxiom)))
+  = pack_turnstile (QLambda (QLambda (QLambda QAxiom)))
 
 let test_anif ()
   : qBool ⊩ anif
   by (simplify_via_norm ())
-  = mk_dturniqet (fun _ -> QIf QTrue QFalse QTrue)
+  = pack_turnstile (QIf QTrue QFalse QTrue)
 
 let test_negb ()
   : (qBool ^-> qBool) ⊩ negb
   by (simplify_via_norm ())
-  = mk_dturniqet (fun _ -> QLambda (QIf QAxiom QFalse QTrue))
+  = pack_turnstile (QLambda (QIf QAxiom QFalse QTrue))
 
 let test_negb_pred ()
   : ((qBool ^-> qBool) ^-> qBool ^-> qBool) ⊩ negb_pred
   by (simplify_via_norm ())
-  = mk_dturniqet (fun _ -> QLambda (QLambda (QIf (QApp qVar1 QAxiom) QFalse QTrue)))
+  = pack_turnstile (QLambda (QLambda (QIf (QApp qVar1 QAxiom) QFalse QTrue)))
 
 let test_if2 ()
   : (qBool ^-> qBool ^-> qBool) ⊩ if2
   by (simplify_stack_ops (); simplify_via_norm ())
-  = mk_dturniqet (fun _ -> QLambda (QLambda (QIf qVar1 QFalse QAxiom)))
+  = pack_turnstile (QLambda (QLambda (QIf qVar1 QFalse QAxiom)))
 
 let test_callback_return ()
   : (qBool ^-> (qBool ^-> qBool)) ⊩ callback_return
   by (simplify_via_norm ())
-  = mk_dturniqet (fun _ -> QLambda (QIf QAxiom
+  = pack_turnstile (QLambda (QIf QAxiom
                  (QLambda qVar1)
                  (QLambda QAxiom)))
 
 let test_callback_return' ()
   : (qBool ^-> (qBool ^-> qBool)) ⊩ callback_return'
   by (simplify_via_norm ())
-  = mk_dturniqet (fun _ -> QLambda (QIf QAxiom
+  = pack_turnstile (QLambda (QIf QAxiom
                  (QLambda qVar1)
                  (QLambda QAxiom)))
 
 let test_make_pair ()
   : (qBool ^-> qBool ^-> (qBool ^* qBool)) ⊩ make_pair
   by (simplify_via_norm ())
-  = mk_dturniqet (fun _ -> QLambda (QLambda (QMkpair qVar1 QAxiom)))
+  = pack_turnstile (QLambda (QLambda (QMkpair qVar1 QAxiom)))
 
 [@@ (preprocess_with simplify_qType)]
 let test_pair_of_functions ()
   : Tot (((qBool ^-> qBool) ^* (qBool ^-> qBool ^-> qBool))
                             ⊩ pair_of_functions)
   by (simplify_stack_ops (); simplify_via_norm ())
-  = mk_dturniqet (fun _ ->  QMkpair
+  = pack_turnstile (QMkpair
       (QLambda (QApp
                   (QLambda (QIf QAxiom QFalse QTrue))
                   QAxiom))
@@ -190,39 +190,39 @@ let test_pair_of_functions2 ()
   : (((qBool ^-> qBool) ^* (qBool ^-> qBool ^-> qBool))
     ⊩ pair_of_functions2)
   by (simplify_via_norm ())
-  = mk_dturniqet (fun _ -> QMkpair
+  = pack_turnstile (QMkpair
       (QLambda (QIf QAxiom QFalse QTrue))
       (QLambda (QLambda (QIf qVar1 QFalse QAxiom))))
 
 let test_fst_pair ()
   : (qBool) ⊩ fst_pair
   by (simplify_via_norm ())
-  = mk_dturniqet (fun _ -> (QFst (QMkpair QTrue Qtt)))
+  = pack_turnstile (QFst (QMkpair QTrue Qtt))
 
 let test_wrap_fst ()
   : ((qBool ^* qBool) ^-> qBool) ⊩ wrap_fst
   by (simplify_via_norm ())
-  = mk_dturniqet (fun _ -> QLambda (QFst QAxiom))
+  = pack_turnstile (QLambda (QFst QAxiom))
 
 let test_wrap_fst_pa ()
   : ((qBool ^* qBool) ^-> qBool) ⊩ wrap_fst_pa
   by (simplify_via_norm ())
-  = mk_dturniqet (fun _ -> QLambda (QFst QAxiom))
+  = pack_turnstile (QLambda (QFst QAxiom))
 
 let test_snd_pair ()
   : (qUnit) ⊩ snd_pair
   by (simplify_via_norm ())
-  = mk_dturniqet (fun _ -> (QSnd (QMkpair QTrue Qtt)))
+  = pack_turnstile (QSnd (QMkpair QTrue Qtt))
 
 let test_wrap_snd ()
   : ((qBool ^* qUnit) ^-> qUnit) ⊩ wrap_snd
   by (simplify_via_norm ())
-  = mk_dturniqet (fun _ -> QLambda (QSnd QAxiom))
+  = pack_turnstile (QLambda (QSnd QAxiom))
 
 let test_wrap_snd_pa ()
   : ((qBool ^* qUnit) ^-> qUnit) ⊩ wrap_snd_pa
   by (simplify_via_norm ())
-  = mk_dturniqet (fun _ -> QLambda (QSnd QAxiom))
+  = pack_turnstile (QLambda (QSnd QAxiom))
 
 let qLet #g (#a #b:qType) #wpx #wpf (#x:fs_oval g a wpx) (#f:fs_oval (extend a g) b wpf)
   (qx : typing g x) (qf : typing _ f)
@@ -235,7 +235,7 @@ let three_lets : bool -> unit =
  let test_three_lets ()
    : (qBool ^-> qUnit) ⊩ three_lets
    by (simplify_via_norm ())
-   = mk_dturniqet (fun _ -> QLambda
+   = pack_turnstile (QLambda
       (qLet (QMkpair QAxiom QAxiom)
       (qLet (QWeaken QAxiom)
       (qLet (QFst qVar1)
@@ -244,35 +244,35 @@ let three_lets : bool -> unit =
 let test_inl_true ()
   : (qBool ^+ qUnit) ⊩ inl_true
    by (simplify_via_norm ())
-  = mk_dturniqet (fun _ -> QInl QTrue)
+  = pack_turnstile (QInl QTrue)
 
 let test_inr_unit ()
   : (qBool ^+ qUnit) ⊩ inr_unit
    by (simplify_via_norm ())
-  = mk_dturniqet (fun _ -> QInr Qtt)
+  = pack_turnstile (QInr Qtt)
 
 [@@ (preprocess_with simplify_qType)]
 let test_return_either ()
   : (qBool ^-> (qUnit ^+ qUnit)) ⊩ return_either
   by (simplify_via_norm ())
-  = mk_dturniqet (fun _ -> QLambda (QIf QAxiom (QInl Qtt) (QInr Qtt)))
+  = pack_turnstile (QLambda (QIf QAxiom (QInl Qtt) (QInr Qtt)))
 
 [@@ (preprocess_with simplify_qType)]
 let test_match_either ()
   : ((qBool ^+ qBool) ^-> qBool) ⊩ match_either
   by (simplify_via_norm ())
-  = mk_dturniqet (fun _ -> QLambda (QCase QAxiom QAxiom QAxiom))
+  = pack_turnstile (QLambda (QCase QAxiom QAxiom QAxiom))
 
 [@expect_failure]
 let test_match_either'
   : ((qBool ^+ qBool) ^-> qBool) ⊩ match_either'
-  = mk_dturniqet (fun _ -> QLambda (QCase QAxiom QAxiom QAxiom))
+  = pack_turnstile (QLambda (QCase QAxiom QAxiom QAxiom))
 
 [@@ (preprocess_with simplify_qType)]
 let test_match_either_arg ()
   : (((qBool ^+ qBool) ^-> qBool ^-> qBool) ⊩ match_either_arg)
   by (simplify_via_norm ())
-  = mk_dturniqet (fun _ -> QLambda (QLambda (
+  = pack_turnstile (QLambda (QLambda (
        QCase
          qVar1
          QAxiom
@@ -324,34 +324,34 @@ open ExamplesIO
 let test_u_return ()
   : (qUnit ^->!@ qBool) ⊩ u_return
   by (simplify_via_norm ())
-  = mk_dturniqet (fun _ -> QLambdaIO (QReturn QTrue))
+  = pack_turnstile (QLambdaIO (QReturn QTrue))
 
 let test_apply_io_return ()
   : (qBool ^->!@ qBool) ⊩ apply_io_return
   by (simplify_via_norm ())
-  = mk_dturniqet (fun _ -> QLambdaIO (QReturn QAxiom))
+  = pack_turnstile (QLambdaIO (QReturn QAxiom))
 
 [@@ (preprocess_with simplify_qType)]
 let test_apply_read ()
   : (qFileDescr ^->!@ (qResexn qString)) ⊩ apply_read
   by (simplify_stack_ops (); norm [delta_only [`%fs_oval_helper;`%apply_read];iota]; simplify_via_norm ())
-  = mk_dturniqet (fun _ -> QLambdaIO (QCall ORead QAxiom))
+  = pack_turnstile (QLambdaIO (QCall ORead QAxiom))
 
 let test_apply_write_const ()
   : (qFileDescr ^->!@ (qResexn qUnit)) ⊩ apply_write_const
   by (simplify_via_norm ())
-  = mk_dturniqet (fun _ -> QLambdaIO (QCall OWrite (QMkpair QAxiom (QStringLit "hello"))))
+  = pack_turnstile (QLambdaIO (QCall OWrite (QMkpair QAxiom (QStringLit "hello"))))
 
 let test_apply_write ()
   : (qFileDescr ^-> qString ^->!@ (qResexn qUnit)) ⊩ apply_write
   by (simplify_via_norm ())
-  = mk_dturniqet (fun _ -> QLambda (QLambdaIO (QCall OWrite (QMkpair (QWeaken QAxiom) QAxiom))))
+  = pack_turnstile (QLambda (QLambdaIO (QCall OWrite (QMkpair (QWeaken QAxiom) QAxiom))))
 
 let test_apply_io_bind_const ()
   : (qUnit ^->!@ qBool) ⊩ apply_io_bind_const
 
   by (simplify_via_norm ())
-  = mk_dturniqet (fun _ -> QLambdaIO (
+  = pack_turnstile (QLambdaIO (
       QBind
         (QReturn QTrue)
         (QReturn QAxiom)))
@@ -359,7 +359,7 @@ let test_apply_io_bind_const ()
 let test_apply_io_bind_identity ()
   : (qBool ^->!@ qBool) ⊩ apply_io_bind_identity
   by (simplify_via_norm ())
-  = mk_dturniqet (fun _ -> QLambdaIO
+  = pack_turnstile (QLambdaIO
       (QBind
         (QReturn QAxiom)
         (QReturn QAxiom)))
@@ -368,7 +368,7 @@ let test_apply_io_bind_identity ()
 let test_apply_io_bind_pure_if ()
   : Tot ((qBool ^->!@ qBool) ⊩ apply_io_bind_pure_if)
   by (simplify_via_norm ())
-  = mk_dturniqet (fun _ -> QLambdaIO
+  = pack_turnstile (QLambdaIO
       (QBind
         (QReturn QAxiom)
         (QIfIO QAxiom
@@ -379,7 +379,7 @@ let test_apply_io_bind_pure_if ()
 let test_apply_io_bind_write ()
   : (qFileDescr ^-> qString ^->!@ (qResexn qUnit)) ⊩ apply_io_bind_write
   by (simplify_via_norm ())
-  = mk_dturniqet (fun _ -> QLambda (QLambdaIO (
+  = pack_turnstile (QLambda (QLambdaIO (
       QBind
          (QReturn QAxiom)
          (QCall OWrite (QMkpair (QWeaken (QWeaken QAxiom)) QAxiom)))))
@@ -388,7 +388,7 @@ let test_apply_io_bind_write ()
 let test_apply_io_bind_read_write ()
   : (qFileDescr ^-> qFileDescr ^->!@ (qResexn qUnit)) ⊩ apply_io_bind_read_write
   by ( simplify_stack_ops (); simplify_via_norm ())
-  = mk_dturniqet (fun _ -> QLambda (QLambdaIO (QBind (QCall ORead (QWeaken QAxiom))
+  = pack_turnstile (QLambda (QLambdaIO (QBind (QCall ORead (QWeaken QAxiom))
     (QCaseIO QAxiom
       (QCall OWrite (QMkpair (QWeaken (QWeaken QAxiom)) (QStringLit "data")))
       (QReturn (QInr QAxiom))))))
@@ -397,7 +397,7 @@ let test_apply_io_bind_read_write ()
 let test_apply_io_bind_read_write' ()
    : (qFileDescr ^-> qFileDescr ^->!@ (qResexn qUnit)) ⊩ apply_io_bind_read_write'
    by (simplify_via_norm ())
-   = mk_dturniqet (fun _ -> QLambda (QLambdaIO (
+   = pack_turnstile (QLambda (QLambdaIO (
        QBind (QCall ORead (QWeaken QAxiom))
          (QCaseIO QAxiom
            (QCall OWrite (QMkpair (QWeaken (QWeaken QAxiom)) (QStringLit "data")))
@@ -407,7 +407,7 @@ let test_apply_io_bind_read_write' ()
 let test_apply_io_bind_read_if_write ()
   : (qFileDescr ^-> qFileDescr ^->!@ (qResexn qUnit)) ⊩ apply_io_bind_read_if_write
   by (simplify_via_norm ())
-  = mk_dturniqet (fun _ -> QLambda (QLambdaIO
+  = pack_turnstile (QLambda (QLambdaIO
       (QBind
         (QCall ORead (QWeaken QAxiom))
          (QCaseIO QAxiom
@@ -417,55 +417,55 @@ let test_apply_io_bind_read_if_write ()
 let test_sendError400 ()
   : (qFileDescr ^->!@ qUnit) ⊩ sendError400
   by (simplify_via_norm ())
-  = mk_dturniqet (fun _ -> QLambdaIO
+  = pack_turnstile (QLambdaIO
       (QBind
         (QCall OWrite (QMkpair QAxiom (QStringLit "error400")))
         (QReturn Qtt)))
 
 let test_const_str
   : qString ⊩ const_str
-  = mk_dturniqet (fun _ -> QStringLit "constant")
+  = pack_turnstile (QStringLit "constant")
 
 let test_greeting ()
   : (qBool ^-> qString) ⊩ greeting
   by (simplify_via_norm ())
-  = mk_dturniqet (fun _ -> QLambda (QIf QAxiom (QStringLit "hello") (QStringLit "goodbye")))
+  = pack_turnstile (QLambda (QIf QAxiom (QStringLit "hello") (QStringLit "goodbye")))
 
 let test_nat_zero
   : qNat ⊩ nat_zero
-  = mk_dturniqet (fun _ -> QZero)
+  = pack_turnstile (QZero)
 
 let test_nat_one
   : qNat ⊩ nat_one
-  = mk_dturniqet (fun _ -> QSucc QZero)
+  = pack_turnstile (QSucc QZero)
 
 let test_nat_two
   : qNat ⊩ nat_two
-  = mk_dturniqet (fun _ -> QSucc (QSucc QZero))
+  = pack_turnstile (QSucc (QSucc QZero))
 
 let test_nat_succ_fn
   : (qNat ^-> qNat) ⊩ nat_succ_fn
-  = mk_dturniqet (fun _ -> QLambda (QSucc QAxiom))
+  = pack_turnstile (QLambda (QSucc QAxiom))
 
 let test_nat_nrec_base ()
   : qNat ⊩ nat_two
-  = mk_dturniqet (fun _ -> QNRec QZero (QSucc (QSucc QZero)) (QLambda (QSucc QAxiom)))
+  = pack_turnstile (QNRec QZero (QSucc (QSucc QZero)) (QLambda (QSucc QAxiom)))
 
 let test_nat_add2 ()
   : (qNat ^-> qNat) ⊩ nat_add2
-  = mk_dturniqet (fun _ -> QLambda (QNRec (QSucc (QSucc QZero)) QAxiom (QLambda (QSucc QAxiom))))
+  = pack_turnstile (QLambda (QNRec (QSucc (QSucc QZero)) QAxiom (QLambda (QSucc QAxiom))))
 
 let test_nat_nrec_two_plus_three1 ()
   : qNat ⊩ nat_five1
-  = mk_dturniqet (fun _ -> QNRec (QSucc (QSucc (QSucc QZero))) (QSucc (QSucc QZero)) (QLambda (QSucc QAxiom)))
+  = pack_turnstile (QNRec (QSucc (QSucc (QSucc QZero))) (QSucc (QSucc QZero)) (QLambda (QSucc QAxiom)))
 
 let test_nat_nrec_two_plus_three2 ()
   : qNat ⊩ nat_five2
-  = mk_dturniqet (fun _ -> QNRec (QSucc (QSucc (QSucc QZero))) (QSucc (QSucc QZero)) (QLambda (QSucc QAxiom)))
+  = pack_turnstile (QNRec (QSucc (QSucc (QSucc QZero))) (QSucc (QSucc QZero)) (QLambda (QSucc QAxiom)))
 
 let test_nat_fact_five ()
   : qNat ⊩ fact_five
-  = mk_dturniqet (fun _ -> QSnd (
+  = pack_turnstile (QSnd (
       QNRec
         (QSucc (QSucc (QSucc (QSucc (QSucc QZero)))))
         (QMkpair QZero (QSucc QZero))
@@ -563,63 +563,63 @@ open ExamplesRefs
 let test_refbool ()
   : qBoolR (fun t -> t == true) ⊩ refbool
   by (simplify_via_norm ())
-  = mk_dturniqet (fun _ -> QRef QTrue #(fun t -> t == true))
+  = pack_turnstile (QRef QTrue #(fun t -> t == true))
 
 let test_falsepre ()
   : (qBoolR (fun _ -> False) ^-> qBool) ⊩ falsepre
   by (simplify_via_norm ())
-  = mk_dturniqet (fun _ -> QLambda (QRef QAxiom #(fun _ -> True)))
+  = pack_turnstile (QLambda (QRef QAxiom #(fun _ -> True)))
 
 let test_just_true ()
   : (qBool ^-> qBoolR (fun x -> x == true)) ⊩ just_true
   by (simplify_via_norm ())
-  = mk_dturniqet (fun _ -> QLambda (QRef QTrue #(fun t -> t == true)))
+  = pack_turnstile (QLambda (QRef QTrue #(fun t -> t == true)))
 
 let test_moving_ref ()
   : (qBoolR (fun _ -> some_ref) ^-> qUnitR (fun _ -> some_ref)) ⊩ moving_ref
   by (simplify_via_norm ())
-  = mk_dturniqet (fun _ -> QLambda (QRef Qtt #(fun _ -> some_ref)))
+  = pack_turnstile (QLambda (QRef Qtt #(fun _ -> some_ref)))
 
 [@@ (preprocess_with simplify_qType)]
 let test_always_false ()
   : (qBool ^-> qBoolR (fun y -> y == false)) ⊩ always_false
   by (simplify_via_norm ())
-  = mk_dturniqet (fun _ -> QLambda (QRef (QIf QAxiom QFalse QAxiom) #(fun t -> t == false)))
+  = pack_turnstile (QLambda (QRef (QIf QAxiom QFalse QAxiom) #(fun t -> t == false)))
 
 [@@ (preprocess_with simplify_qType)]
 let test_always_false_complex ()
   : (qBool ^-> qBoolR (fun y -> y == false)) ⊩ always_false_complex
   by (simplify_via_norm ())
-  = mk_dturniqet (fun _ -> QLambda (QRef (QIf QAxiom (QIf QAxiom QFalse QTrue) QFalse) #(fun t -> t == false)))
+  = pack_turnstile (QLambda (QRef (QIf QAxiom (QIf QAxiom QFalse QTrue) QFalse) #(fun t -> t == false)))
 
 let test_always_false_ho ()
   : ((qUnit ^-> qBoolR (fun x -> x == true)) ^-> qBoolR (fun y -> y == false))
     ⊩ always_false_ho
   by (simplify_via_norm ())
-  = mk_dturniqet (fun _ -> QLambda (QRef (QIf (QRef (QApp QAxiom Qtt) #(fun _ -> True)) QFalse QTrue) #(fun t -> t == false)))
+  = pack_turnstile (QLambda (QRef (QIf (QRef (QApp QAxiom Qtt) #(fun _ -> True)) QFalse QTrue) #(fun t -> t == false)))
 
 [@@ (preprocess_with simplify_qType)]
 let test_if_x ()
   : ((qBoolR (fun x -> x == true) ^-> qBool) ^-> qBool ^-> qBool) ⊩ if_x
   by (simplify_via_norm ())
-  = mk_dturniqet (fun _ -> QLambda (QLambda (QIf QAxiom
+  = pack_turnstile (QLambda (QLambda (QIf QAxiom
       (QApp qVar1 (QRef QAxiom #(fun x -> x == true))) QFalse)))
 
 let test_seq_basic ()
   : ((qUnit ^-> qUnit) ^-> qUnit) ⊩ seq_basic
   by (simplify_via_norm ())
-  = mk_dturniqet (fun _ -> QLambda (qLet (QApp QAxiom Qtt) Qtt))
+  = pack_turnstile (QLambda (qLet (QApp QAxiom Qtt) Qtt))
 
 let test_seq_qref ()
   : ((qUnit ^-> qUnitR (fun _ -> q_ref)) ^-> qUnitR (fun _ -> q_ref)) ⊩ seq_qref
   by (simplify_via_norm ())
-  = mk_dturniqet (fun _ -> QLambda (qLet (QApp QAxiom Qtt) (QRef Qtt #(fun _ -> q_ref))))
+  = pack_turnstile (QLambda (qLet (QApp QAxiom Qtt) (QRef Qtt #(fun _ -> q_ref))))
 
 let test_seq_p_implies_q ()
   : ((qBoolR p_ref ^-> qUnitR (fun _ -> q_ref)) ^-> qBoolR p_ref ^-> qBoolR (fun _ -> q_ref))
     ⊩ seq_p_implies_q
   by (simplify_via_norm ())
-  = mk_dturniqet (fun _ -> QLambda (QLambda
+  = pack_turnstile (QLambda (QLambda
       (qLet (QApp qVar1 QAxiom) (QRef qVar1 #(fun _ -> q_ref)))))
 
 [@@ (preprocess_with simplify_qType)]
@@ -627,7 +627,7 @@ let test_if_seq ()
   : ((qBoolR (fun x -> x == true) ^-> qUnitR (fun _ -> q_ref)) ^-> qBool ^-> qBoolR (fun r -> r == true ==> q_ref))
     ⊩ if_seq
   by (simplify_via_norm ())
-  = mk_dturniqet (fun _ ->
+  = pack_turnstile (
     QLambda (QLambda (
       QIf QAxiom
         (qLet
@@ -640,7 +640,7 @@ let test_context ()
   : (qBool ^-> (qBoolR (fun x -> x == true) ^-> qBool ^-> qBool) ^-> qBool ^-> qBool)
     ⊩ context
   by (simplify_via_norm ())
-  = mk_dturniqet (fun _ -> QLambda (QLambda (
+  = pack_turnstile (QLambda (QLambda (
     QIf qVar1
       (QApp QAxiom (QRef qVar1 #(fun x -> x == true)))
       (QLambda QAxiom))))
@@ -648,7 +648,7 @@ let test_context ()
 // let test_pure_fun ()
 //  : (qArrR (qBoolR (fun b -> b == true)) qBool (fun b r -> r == b)) ⊩ pure_fun
 //   by (simplify_via_norm ())
-//   = mk_dturniqet (fun _ -> QRetype (QLambda #(qBoolR (fun b -> b == true)) QTrue))
+//   = pack_turnstile (QRetype (QLambda #(qBoolR (fun b -> b == true)) QTrue))
 
 #pop-options
 
@@ -703,25 +703,25 @@ open ExamplesIORefinements
 let test_ior_simple_erase_ref ()
   : (qBoolR (fun t -> t == true) ^->!@ qBool) ⊩ simple_erase_ref
   by (simplify_via_norm ())
-  = mk_dturniqet (fun _ -> QLambdaIO (QReturn (QRef QAxiom #(fun _ -> True))))
+  = pack_turnstile (QLambdaIO (QReturn (QRef QAxiom #(fun _ -> True))))
 
 (** Example 2: Preserve refinement in IO *)
 let test_ior_simple_ref_id ()
   : (qBoolR (fun t -> t == true) ^->!@ qBoolR (fun t -> t == true)) ⊩ simple_ref_id
   by (simplify_via_norm ())
-  = mk_dturniqet (fun _ -> QLambdaIO (QReturn QAxiom))
+  = pack_turnstile (QLambdaIO (QReturn QAxiom))
 
 (** Example 3: Weaken refinement in IO *)
 let test_ior_simple_reref_id ()
   : (qBoolR (fun t -> t == true) ^->!@ qBoolR (fun t -> t == true \/ t == false)) ⊩ simple_reref_id
   by (simplify_via_norm ())
-  = mk_dturniqet (fun _ -> QLambdaIO (QReturn (QRef QAxiom #(fun t -> t == true \/ t == false))))
+  = pack_turnstile (QLambdaIO (QReturn (QRef QAxiom #(fun t -> t == true \/ t == false))))
 
 (** Example 4: Bind with IO call, then return refined *)
 let test_ior_simple_ref_bind ()
   : (qBoolR (fun t -> t == true) ^->!@ qBoolR (fun t -> t == true \/ t == false)) ⊩ simple_ref_bind
   by (simplify_stack_ops (); simplify_via_norm ())
-  = mk_dturniqet (fun _ -> QLambdaIO (
+  = pack_turnstile (QLambdaIO (
     QBind
       (QCall OOpen (QStringLit "./string"))
       (QReturn (QRef (QWeaken QAxiom) #(fun t -> t == true \/ t == false)))))
@@ -730,13 +730,13 @@ let test_ior_simple_ref_bind ()
 let test_ior_io_ret_ref_true ()
   : (qUnit ^->!@ qBoolR (fun x -> x == true)) ⊩ io_ret_ref_true
   by (simplify_via_norm ())
-  = mk_dturniqet (fun _ -> QLambdaIO (QReturn (QRef QTrue #(fun x -> x == true))))
+  = pack_turnstile (QLambdaIO (QReturn (QRef QTrue #(fun x -> x == true))))
 
 (** Example 7: Return refined false constant *)
 let test_ior_io_ret_ref_false ()
   : (qUnit ^->!@ qBoolR (fun x -> x == false)) ⊩ io_ret_ref_false
   by (simplify_via_norm ())
-  = mk_dturniqet (fun _ -> QLambdaIO (QReturn (QRef QFalse #(fun x -> x == false))))
+  = pack_turnstile (QLambdaIO (QReturn (QRef QFalse #(fun x -> x == false))))
 
 (** Example 8: Negate refined input in IO *)
 
@@ -744,20 +744,20 @@ let test_ior_io_ret_ref_false ()
 let test_ior_io_negate_ref ()
   : (qBoolR (fun x -> x == true) ^->!@ qBoolR (fun y -> y == false)) ⊩ io_negate_ref
   by (simplify_via_norm ())
-  = mk_dturniqet (fun _ -> QLambdaIO (QReturn (
+  = pack_turnstile (QLambdaIO (QReturn (
       QRef (QIf (QRef QAxiom) QFalse QTrue) #(fun x -> x == false))))
 
 (** Example 9: If-then-else with both branches false *)
 let test_ior_io_if_both_false ()
   : (qBool ^->!@ qBoolR (fun y -> y == false)) ⊩ io_if_both_false
   by (simplify_via_norm ())
-  = mk_dturniqet (fun _ -> QLambdaIO (QReturn (QRef (QIf QAxiom QFalse QFalse) #(fun x -> x == false))))
+  = pack_turnstile (QLambdaIO (QReturn (QRef (QIf QAxiom QFalse QFalse) #(fun x -> x == false))))
 
 (** Example 10: Bind with unit, then return refined *)
 let test_ior_io_bind_ret_ref ()
   : (qUnit ^->!@ qBoolR (fun x -> x == true)) ⊩ io_bind_ret_ref
   by (simplify_via_norm ())
-  = mk_dturniqet (fun _ -> QLambdaIO (
+  = pack_turnstile (QLambdaIO (
     QBind
       (QReturn Qtt)
       (QReturn (QRef QTrue #(fun x -> x == true)))))
@@ -766,7 +766,7 @@ let test_ior_io_bind_ret_ref ()
 let test_ior_io_call_ret_ref ()
   : (qUnit ^->!@ qBoolR (fun y -> y == true)) ⊩ io_call_ret_ref
   by (simplify_via_norm ())
-  = mk_dturniqet (fun _ -> QLambdaIO (
+  = pack_turnstile (QLambdaIO (
       QBind
         (QCall OOpen (QStringLit "./file"))
         (QReturn (QRef QTrue #(fun x -> x == true)))))
@@ -775,7 +775,7 @@ let test_ior_io_call_ret_ref ()
 let test_ior_io_two_calls_ref ()
   : (qUnit ^->!@ qBoolR (fun y -> y == true)) ⊩ io_two_calls_ref
   by (simplify_via_norm ())
-  = mk_dturniqet (fun _ ->
+  = pack_turnstile (
     QLambdaIO (
       QBind
         (QCall OOpen (QStringLit "./a"))
@@ -787,26 +787,26 @@ let test_ior_io_two_calls_ref ()
 let test_ior_io_inl_ref ()
   : (qBoolR (fun x -> x == true) ^->!@ qResexn qBool) ⊩ io_inl_ref
   by (simplify_via_norm ())
-  = mk_dturniqet (fun _ -> QLambdaIO (QReturn (QInl (QRef QAxiom))))
+  = pack_turnstile (QLambdaIO (QReturn (QInl (QRef QAxiom))))
 
 (** Example 14: Inject Inr (error) in IO *)
 let test_ior_io_inr_ref ()
   : (qUnit ^->!@ qResexn qBool) ⊩ io_inr_ref
   by (simplify_via_norm ())
-  = mk_dturniqet (fun _ -> QLambdaIO (QReturn (QInr Qtt)))
+  = pack_turnstile (QLambdaIO (QReturn (QInr Qtt)))
 
 (** Example 15: Return pair with refined input in IO *)
 let test_ior_io_pair_ref ()
   : (qBoolR (fun x -> x == true) ^->!@ (qBool ^* qUnit)) ⊩ io_pair_ref
   by (simplify_via_norm ())
-  = mk_dturniqet (fun _ -> QLambdaIO (QReturn (QMkpair (QRef QAxiom) Qtt)))
+  = pack_turnstile (QLambdaIO (QReturn (QMkpair (QRef QAxiom) Qtt)))
 
 (** Example 16: Case analysis returning refined in IO *)
 [@@ (preprocess_with simplify_qType)]
 let test_ior_io_case_ref ()
   : ((qBool ^+ qUnit) ^->!@ qBoolR (fun y -> y == false)) ⊩ io_case_ref
   by (simplify_via_norm ())
-  = mk_dturniqet (fun _ -> QLambdaIO (
+  = pack_turnstile (QLambdaIO (
       QCaseIO QAxiom
         (QReturn (QRef QFalse #(fun y -> y == false)))
         (QReturn (QRef QFalse #(fun y -> y == false)))))
@@ -816,7 +816,7 @@ let test_ior_io_case_ref ()
 let test_ior_io_ifbang_ref ()
   : (qBool ^->!@ qBoolR (fun y -> y == true)) ⊩ io_ifbang_ref
   by (simplify_via_norm ())
-  = mk_dturniqet (fun _ -> QLambdaIO (
+  = pack_turnstile (QLambdaIO (
       QBind
         (QReturn QAxiom)
         (QIfIO QAxiom
@@ -828,7 +828,7 @@ let test_ior_io_ifbang_ref ()
 let test_ior_io_matchbang_ref ()
   : (qUnit ^->!@ qBoolR (fun y -> y == true \/ y == false)) ⊩ io_matchbang_ref
   by (simplify_via_norm ())
-  = mk_dturniqet (fun _ ->
+  = pack_turnstile (
     QLambdaIO (
       QBind
         (QCall OOpen (QStringLit "./file"))
@@ -840,14 +840,14 @@ let test_ior_io_matchbang_ref ()
 let test_ior_io_ghost_seq ()
   : ((qUnit ^-> qUnitR (fun _ -> ExamplesIORefinements.q_ref)) ^->!@ qUnitR (fun _ -> ExamplesIORefinements.q_ref)) ⊩ io_ghost_seq
   by (simplify_via_norm ())
-  = mk_dturniqet (fun _ -> QLambdaIO (
+  = pack_turnstile (QLambdaIO (
     QReturn (qLet (QApp QAxiom Qtt) (QRef Qtt))))
 
 (** Example 20: Apply refined callback in IO *)
 let test_ior_io_apply_callback ()
   : ((qBoolR (fun x -> x == true) ^-> qBool) ^->!@ qBool) ⊩ io_apply_callback
   by (simplify_via_norm ())
-  = mk_dturniqet (fun _ ->
+  = pack_turnstile (
     QLambdaIO (QReturn (QApp QAxiom (QRef QTrue #(fun x -> x == true)))))
 
 (** Example 21: Validate with refined callback in IO *)
@@ -857,7 +857,7 @@ let test_ior_io_apply_callback ()
 let test_ior_pure_validate ()
   : (qString ^-> (qArrR qString qBool (fun x y -> y ==> valid x)) ^-> qResexn (qStringR (fun x -> valid x))) ⊩ pure_validate
  by (simplify_via_norm ())
-  = mk_dturniqet (fun _ ->
+  = pack_turnstile (
       QLambda (QLambda (
         (QIf (QApp QAxiom (QWeaken QAxiom))
             (QInl (QRetype (QWeaken QAxiom)))
@@ -867,7 +867,7 @@ let test_ior_pure_validate ()
 let test_ior_io_validate_simp ()
   : (qString ^-> (qArrR qString qBool (fun x y -> y ==> valid x)) ^->!@ qResexn (qStringR (fun x -> valid x))) ⊩ io_validate_simp
  by (simplify_stack_ops (); simplify_via_norm ())
-  = mk_dturniqet (fun _ ->
+  = pack_turnstile (
       QLambda (QLambdaIO (
         (QReturn
           (QIf (QApp QAxiom (QWeaken QAxiom))
@@ -879,7 +879,7 @@ let test_ior_io_validate_simp ()
 // let test_ior_io_validate ()
 //   : ((qArrR qString qBool (fun x y -> y ==> valid x)) ^->!@ qResexn (qStringR (fun x -> valid x))) ⊩ io_validate
 //   by (simplify_stack_ops (); simplify_via_norm ())
-//   = mk_dturniqet (fun _ ->
+//   = pack_turnstile (
 //     QLambdaIO (
 //       QBind (QCall OOpen (QStringLit "./file"))
 //         (QCaseIO QAxiom
